\begin{topic}{young-diagram}{Young diagram}
    Given a partition $\lambda = (\lambda_1, \lambda_2, \ldots, \lambda_k)$ of a non-negative integer $n \ge 0$, a \textbf{Young diagram} of shape $\lambda$ is a collection of $n$ boxes, arranged in left-aligned rows, such that row $i$ has $\lambda_i$ boxes. For example, a Young diagram of shape $(5, 3, 2)$ is given by:
    \[ \begin{tikzpicture}
        \begin{scope}[scale=0.5]
            \draw (0, 3) -- (5, 3); \draw (0, 2) -- (5, 2); \draw (0, 1) -- (3, 1); \draw (0, 0) -- (2, 0); \draw (0, 3) -- (0, 0); \draw (1, 3) -- (1, 0); \draw (2, 3) -- (2, 0); \draw (3, 3) -- (3, 1); \draw (4, 3) -- (4, 2); \draw (5, 3) -- (5, 2);
        \end{scope}
    \end{tikzpicture} \]
    The \textit{arm length} of a box $s$, denoted $a_\lambda(s)$, is the number of boxes to the right of $s$. The \textit{leg length} of $s$, denoted $l_\lambda(s)$, is the number of boxes below $s$.
    
    A \textbf{Young tableau} is obtained from a Young diagram by filling in the boxes with numbers. A Young tableau is \textbf{standard} if the entries in each row and each column are increasing.
\end{topic}

\begin{topic}{generating-function}{generating function}
    The \textbf{generating function} of a sequence $a_0, a_1, a_2, \ldots$ in a \tref{AA:ring}{commutative ring} $R$ is the formal power series
    \[ \sum_{n = 0}^{\infty} a_n t^n = a_0 + a_1 t + a_2 t^2 + \cdots \in R \llbracket t \rrbracket . \]
\end{topic}

\begin{example}{generating-function}
    \begin{itemize}
        \item The generating function of the constant sequence $1, 1, 1, \ldots$ is
        \[ \sum_{n = 0}^{\infty} t^n = \frac{1}{1 - t} . \]
        \item The generating function of the linear sequence $0, 1, 2, 3, \ldots$ is
        \[ \sum_{n = 0}^{\infty} n t^{n} = t \cdot \frac{d}{dt} \sum_{n = 0}^{\infty} t^{n} = t \cdot \frac{d}{dt} \left( \frac{1}{1 - t} \right) = \frac{t}{(1 - t)^2} . \]
        % \item The generating function of 
    \end{itemize}
\end{example}

\begin{example}{generating-function}
    Assuming $R$ has \tref{AA:characteristic}{characteristic} zero, the sequence can be obtained from the generating function $F \in R \llbracket t \rrbracket$ as follows. Writing
    \[ F = \sum_{n = 0}^{\infty} a_n t^n = a_0 + a_1 t + a_2 t^2 + \cdots , \]
    we obtain the coefficients $a_n$ from the $n$-th derivatives of $F$ as
    \[ a_n = \frac{F^{(n)}(0)}{n!} . \]
\end{example}

\begin{topic}{mobius-function}{Möbius function}
    The \textbf{Möbius function} $\mu$ is the function that assigns to any positive integer $n > 0$ the value
    \[ \mu(n) = \sum_{\substack{1 \le k \le n \\ \gcd(k, n) = 1}} e^{2\pi i \frac{k}{n}} , \]
    or alternatively,
    \[ \mu(n) = \left\{ \begin{array}{cl}
         +1 & \textup{ if $n$ is square-free with even number of prime factors}, \\
         -1 & \textup{ if $n$ is square-free with odd number of prime factors}, \\
         0 & \textup{ if $n$ has a squared prime factor}.
    \end{array} \right. \]
\end{topic}

\begin{example}{mobius-function}
    The first few values of $\mu$ are given by
    \[ \begin{array}{lllll}
        \mu(1) = 1, & \mu(2) = -1, & \mu(3) = -1, & \mu(4) = 0, & \mu(5) = -1, \\
        \mu(6) = 1, & \mu(7) = -1, & \mu(8) = 0, & \mu(9) = 0, & \mu(10) = 1, \ldots
    \end{array} \]
\end{example}

\begin{topic}{cantor-theorem}{Cantor's theorem}
    \textbf{Cantor's theorem} states that the cardinality of a set $A$ is always strictly smaller than the cardinality of its power set $\mathcal{P}(A)$.
\end{topic}

\begin{example}{cantor-theorem}
    \begin{proof}
        The cardinality of $A$ is at most the cardinality of $\mathcal{P}(A)$ since $x \mapsto \{ x \}$ is an injection $A \to \mathcal{P}(A)$.
        Conversely, suppose that there exists a surjective function $f : A \to \mathcal{P}(A)$, and let $B = \{ x \in A \;|\; x \not\in f(x) \}$. Then by surjectivity of $f$ there exists some $y \in A$ such that $f(y) = B$. But then $y \in B$ if and only if $y \not\in f(y) = B$, which is a contradiction. Therefore, the cardinality of $A$ is strictly smaller than that of $\mathcal{P}(A)$.
    \end{proof}
\end{example}

\begin{topic}{schur-function}{Schur function}
    Let $n$ be a positive integer. Write $a_\alpha = \det(x_i^{\alpha_j})_{i, j = 1}^{n}$ for any sequence $\alpha = (\alpha_1, \ldots, \alpha_n)$. For any partition $\lambda = (\lambda_1, \ldots, \lambda_n)$ of length at most $n$, the \textbf{Schur polynomial} of $\lambda$ is the \tref{AA:symmetric-polynomial}{polynomial}
    \[ s_\lambda = a_{\lambda + \delta} / a_\delta \in \ZZ[x_1, \ldots, x_n] , \]
    where $\delta = (n - 1, n - 2, \ldots, 1, 0)$.
    
    In passing from $n$ to $n + 1$, it can be seen that $s_\lambda(x_1, x_2, \ldots, x_n, 0) = s_\lambda(x_1, x_2, \ldots, x_n)$. Hence, there is a uniquely defined element
    \[ s_\lambda \in \Lambda := \bigoplus_{r \ge 0} \Lambda^r , \quad \textup{ where  } \Lambda^r = \varprojlim_n \ZZ[x_1, \ldots, x_n]_{(r)}^{S_n} , \]
    called the \textbf{Schur function} of $\lambda$.
\end{topic}

\begin{example}{schur-function}
    For $n = 3$, we have
    \begin{itemize}
        \item $s_{(0, 0, 0)} = 1$,
        \item $s_{(1, 0, 0)} = x_1 + x_2 + x_3$,
        \item $s_{(1, 1, 0)} = x_1 x_2 + x_1 x_3 + x_2 x_3$,
        \item $s_{(1, 1, 1)} = x_1 x_2 x_3$,
        \item $s_{(2, 0, 0)} = x_1^2 + x_1 x_2 + x_1 x_3 + x_2^2 + x_2 x_3 + x_3^2$,
        \item $s_{(2, 1, 0)} = (x_1 + x_2) (x_1 + x_3) (x_2 + x_3)$.
    \end{itemize}
    For any $n \ge 1$ and $\lambda = (1, 0, 0, \ldots)$, we have $s_\lambda = \sum_{i = 1}^{n} x_i$, so we obtain the Schur function $s_\lambda = \sum_{i = 1}^{\infty} x_i \in \Lambda$.
\end{example}

% \begin{topic}{macdonald-polynomials}{Macdonald polynomials}
%     Let $q$ and $t$ be two parameters.
    
%     The \textbf{Macdonald polynomials} are a family of polynomials $P_\lambda(q, t)$ uniquely determined by the conditions
%     \[ P_\lambda(q, t) = m_\lambda + \sum_{\mu < \lambda} m_\mu \]
%     \[ \langle P_\lambda, P_\mu \rangle_{q, t} = 0 \quad \textup{ for } \lambda \ne \mu . \]
%     where
%     \[ \langle p_\lambda, p_\mu \rangle = \delta_{\lambda \mu} z_\lambda \prod_{i = 1}^{\ell(\lambda)} \frac{1 - q^{\lambda_i}}{1 - t^{\lambda_i}} . \]
% \end{topic}
